
<style>
html, body {
    font : 20pt monospace;
}
body {
    text-align: center;
}
</style>

# Algebra 101

$$
\begin{aligned}
& (a+b)^2=a^2+2 a b+b^2 \\
& (a-b)^2=a^2-2 a b+b^2 \\
& (a+b)^3=a^3+3 a^2 b+3 a b^2+b^3 \\
& a^3+b^3=(a+b)\left(a^2-a b+b^2\right) \\
& a^3-b^3=(a-b)\left(a^2+a b+b^2\right) \\
& a^2+b^2=(a+b)^2-2 a b \\
& a^2-b^2=(a+b)(a-b) \\
& a+b=\frac{a^3+b^3}{a^2-a b+b^2} \\
& a-b=\frac{a^3-b^3}{a^2+a b+b^2} \\
& (a+b)^4=a^4+4 a^3 b+6 a^2 b^2-4 a b^3+b^4 \\
& (a-b)^4=a^4-4 a^3 b+6 a^2 b^2-4 a b^3+b^4 \\
& a^4+b^4=\left(a^2+b^2\right)^2-2 a^2 b^2 \\
& a^4-b^4=(a+b)(a-b)\left(a^2+b^2\right)
\end{aligned}
$$